use indexr for all envs

dev2016/fsub.v
@@ -32,63 +32,39 @@ Inductive ty : Type :=
 
 Inductive tm : Type :=
 | tvar : id -> tm
-| tabs : id -> ty -> tm -> tm
+| tabs : ty -> tm -> tm
 | tapp : tm -> tm -> tm
-| ttabs : id -> ty -> tm -> tm
+| ttabs : ty -> tm -> tm
 | ttapp : tm -> ty -> tm
 .
 
 Inductive vl : Type :=
 (* a closure for a term abstraction *)
-| vabs : list (id*vl) (*H*) -> id -> ty -> tm -> vl
+| vabs : list vl (*H*) -> ty -> tm -> vl
 (* a closure for a type abstraction *)
-| vtabs : list (id*vl) (*H*) -> id -> ty -> tm -> vl
+| vtabs : list vl (*H*) -> ty -> tm -> vl
 (* For uniformity, we represent a type closing over H here as well,
    because such types can be bound in H during type application.
    They represent a type variable binding in the runtime environment,
    corresponding to TMem in the static environment.
 *)
-| vty : list (id*vl) (*H*) -> ty -> vl
+| vty : list vl (*H*) -> ty -> vl
 .
 
-Definition tenv := list (id*ty). (* Gamma environment: static *)
-Definition venv := list (id*vl). (* H environment: run-time *)
-Definition aenv := list (id*(venv*ty)). (* J environment: abstract at run-time *)
+Definition tenv := list ty. (* Gamma environment: static *)
+Definition venv := list vl. (* H environment: run-time *)
+Definition aenv := list (venv*ty). (* J environment: abstract at run-time *)
 
 (* ### Representation of Bindings ### *)
 
-(* An environment is a list of strictly decreasing ids. *)
+(* An environment is a list of values, indexed by decrementing ids. *)
 
-Fixpoint fresh {X: Type} (l : list (id * X)): nat :=
-  match l with
-    | [] => 0
-    | (n',a)::l' => 1 + n'
-  end.
-
-Fixpoint index {X : Type} (n : id) (l : list (id * X)) : option X :=
+Fixpoint indexr {X : Type} (n : id) (l : list X) : option X :=
   match l with
     | [] => None
-    | (n',a) :: l'  =>
-      if le_lt_dec (fresh l') n' then
-        if (beq_nat n n') then Some a else index n l'
-      else None
-  end.
-
-(* An indexr'ed environment of size n is a list of strictly decrementing ids,
-   from n-1 to 0.
-   In this case, we don't even look at the id LHS in the environment,
-   but just rely on the list structures.
-   Such rigid environments are used for 'abstract' environments, which the
-   meta-theory fully controls and where there is no need for user-visible
-   flexibility in using ids.
-*)
-Fixpoint indexr {X : Type} (n : id) (l : list (id * X)) : option X :=
-  match l with
-    | [] => None
-    | (n',a) :: l' =>
+    | a :: l' =>
       if (beq_nat n (length l')) then Some a else indexr n l'
   end.
-
 
 (* closed and open define a locally-nameless encoding wrt to TVarB type variables. *)
 Inductive closed_rec: nat -> nat -> ty -> Prop :=
@@ -134,9 +110,9 @@ Definition open u T := open_rec 0 u T.
 Fixpoint open_tm_rec (k: nat) (u: ty) (t: tm) { struct t }: tm :=
   match t with
     | tvar x => tvar x
-    | tabs x T t => tabs x (open_rec k u T) (open_tm_rec (S k) u t)
+    | tabs T t => tabs (open_rec k u T) (open_tm_rec (S k) u t)
     | tapp t1 t2 => tapp (open_tm_rec k u t1) (open_tm_rec k u t2)
-    | ttabs x T t => ttabs x (open_rec k u T) (open_tm_rec (S k) u t)
+    | ttabs T t => ttabs (open_rec k u T) (open_tm_rec (S k) u t)
     | ttapp t1 T2 => ttapp (open_tm_rec k u t1) (open_rec k u T2)
   end.
 
@@ -189,12 +165,12 @@ Inductive stp: tenv -> tenv -> ty -> ty -> Prop :=
     stp G1 GH T1 T2 ->
     stp G1 GH (TMem T1) (TMem T2)
 | stp_sel1: forall G1 GH T T2 x,
-    index x G1 = Some (TMem T) ->
+    indexr x G1 = Some (TMem T) ->
     closed 0 0 T ->
     stp G1 GH T T2 ->
     stp G1 GH (TVarF x) T2
 | stp_selx: forall G1 GH T x,
-    index x G1 = Some (TMem T) ->
+    indexr x G1 = Some (TMem T) ->
     stp G1 GH (TVarF x) (TVarF x)
 | stp_sela1: forall G1 GH T T2 x,
     indexr x GH = Some (TMem T) ->
@@ -209,35 +185,35 @@ Inductive stp: tenv -> tenv -> ty -> ty -> Prop :=
     x = length GH ->
     closed 1 (length GH) T2 -> (* must not accidentally bind x *)
     closed 1 (length GH) T4 ->
-    stp G1 ((0,TMem T1)::GH) (open (TVarH x) T2) (open (TVarH x) T2) -> (* regularity *)
-    stp G1 ((0,TMem T3)::GH) (open (TVarH x) T2) (open (TVarH x) T4) ->
+    stp G1 ((TMem T1)::GH) (open (TVarH x) T2) (open (TVarH x) T2) -> (* regularity *)
+    stp G1 ((TMem T3)::GH) (open (TVarH x) T2) (open (TVarH x) T4) ->
     stp G1 GH (TAll T1 T2) (TAll T3 T4)
 .
 
 (* ### Type Assignment ### *)
 Inductive has_type : tenv -> tm -> ty -> Prop :=
 | t_var: forall x env T1,
-           index x env = Some T1 ->
+           indexr x env = Some T1 ->
            stp env [] T1 T1 ->
            has_type env (tvar x) T1
 | t_app: forall env f x T1 T2,
            has_type env f (TFun T1 T2) ->
            has_type env x T1 ->
            has_type env (tapp f x) T2
-| t_abs: forall env x y T1 T2,
-           has_type ((x,T1)::env) (open_tm (TVarF x) y) T2 ->
+| t_abs: forall env y T1 T2,
+           has_type (T1::env) (open_tm (TVarF (length env)) y) T2 ->
            stp env [] (TFun T1 T2) (TFun T1 T2) ->
-           fresh env <= x ->
-           has_type env (tabs x T1 y) (TFun T1 T2)
+           has_type env (tabs T1 y) (TFun T1 T2)
 | t_tapp: forall env f T11 T12 T,
            has_type env f (TAll T11 T12) ->
            T = open T11 T12 ->
            has_type env (ttapp f T11) T
-| t_tabs: forall env x y T1 T2,
-           has_type ((x,TMem T1)::env) (open_tm (TVarF x) y) (open (TVarF x) T2) ->
+| t_tabs: forall env y T1 T2,
+            has_type ((TMem T1)::env)
+                     (open_tm (TVarF (length env)) y)
+                     (open (TVarF (length env)) T2) ->
            stp env [] (TAll T1 T2) (TAll T1 T2) ->
-           fresh env <= x ->
-           has_type env (ttabs x T1 y) (TAll T1 T2)
+           has_type env (ttabs T1 y) (TAll T1 T2)
 | t_sub: forall env e T1 T2,
            has_type env e T1 ->
            stp env [] T1 T2 ->
@@ -263,18 +239,18 @@ Inductive stp2: venv -> ty -> venv -> ty -> aenv  -> Prop :=
 (* concrete type variables *)
 (* vty already marks binding as type binding, so need for additional TMem marker *)
 | stp2_sel1: forall G1 G2 GX TX x T2 GH,
-    index x G1 = Some (vty GX TX) ->
+    indexr x G1 = Some (vty GX TX) ->
     closed 0 0 TX ->
     stp2 GX TX G2 T2 GH ->
     stp2 G1 (TVarF x) G2 T2 GH
 | stp2_sel2: forall G1 G2 GX TX x T1 GH,
-    index x G2 = Some (vty GX TX) ->
+    indexr x G2 = Some (vty GX TX) ->
     closed 0 0 TX ->
     stp2 G1 T1 GX TX GH ->
     stp2 G1 T1 G2 (TVarF x) GH
 | stp2_selx: forall G1 G2 v x1 x2 GH,
-    index x1 G1 = Some v ->
-    index x2 G2 = Some v ->
+    indexr x1 G1 = Some v ->
+    indexr x2 G2 = Some v ->
     stp2 G1 (TVarF x1) G2 (TVarF x2) GH
 
 (* abstract type variables *)
@@ -293,18 +269,18 @@ Inductive stp2: venv -> ty -> venv -> ty -> aenv  -> Prop :=
     x = length GH ->
     closed 1 (length GH) T2 -> (* must not accidentally bind x *)
     closed 1 (length GH) T4 ->
-    stp2 G1 (open (TVarH x) T2) G1 (open (TVarH x) T2) ((0,(G1, T1))::GH) -> (* regularity *)
-    stp2 G1 (open (TVarH x) T2) G2 (open (TVarH x) T4) ((0,(G2, T3))::GH) ->
+    stp2 G1 (open (TVarH x) T2) G1 (open (TVarH x) T2) ((G1, T1)::GH) -> (* regularity *)
+    stp2 G1 (open (TVarH x) T2) G2 (open (TVarH x) T4) ((G2, T3)::GH) ->
     stp2 G1 (TAll T1 T2) G2 (TAll T3 T4) GH
 .
 
 (* consistent environment *)
 Inductive wf_env : venv -> tenv -> Prop :=
 | wfe_nil : wf_env nil nil
-| wfe_cons : forall n v t vs ts,
-    val_type ((n,v)::vs) v t ->
+| wfe_cons : forall v t vs ts,
+    val_type (v::vs) v t ->
     wf_env vs ts ->
-    wf_env (cons (n,v) vs) (cons (n,t) ts)
+    wf_env (cons v vs) (cons t ts)
 
 (* value type assignment *)
 with val_type : venv -> vl -> ty -> Prop :=
@@ -314,23 +290,23 @@ with val_type : venv -> vl -> ty -> Prop :=
     val_type env (vty venv T1) TE
 | v_abs: forall env venv tenv x y T1 T2 TE,
     wf_env venv tenv ->
-    has_type ((x,T1)::tenv) (open_tm (TVarF x) y) T2 ->
-    fresh venv <= x ->
+    has_type (T1::tenv) (open_tm (TVarF x) y) T2 ->
+    length venv = x ->
     stp2 venv (TFun T1 T2) env TE [] ->
-    val_type env (vabs venv x T1 y) TE
+    val_type env (vabs venv T1 y) TE
 | v_tabs: forall env venv tenv x y T1 T2 TE,
     wf_env venv tenv ->
-    has_type ((x,TMem T1)::tenv) (open_tm (TVarF x) y) (open (TVarF x) T2) ->
-    fresh venv <= x ->
+    has_type ((TMem T1)::tenv) (open_tm (TVarF x) y) (open (TVarF x) T2) ->
+    length venv = x ->
     stp2 venv (TAll T1 T2) env TE [] ->
-    val_type env (vtabs venv x T1 y) TE
+    val_type env (vtabs venv T1 y) TE
 .
 
 Inductive wf_envh : venv -> aenv -> tenv -> Prop :=
 | wfeh_nil : forall vvs, wf_envh vvs nil nil
-| wfeh_cons : forall n t vs vvs ts,
+| wfeh_cons : forall t vs vvs ts,
     wf_envh vvs vs ts ->
-    wf_envh vvs (cons (n,(vvs,t)) vs) (cons (n,TMem t) ts)
+    wf_envh vvs (cons (vvs,t) vs) (cons (TMem t) ts)
 .
 
 Inductive valh_type : venv -> aenv -> (venv*ty) -> ty -> Prop :=
@@ -353,9 +329,9 @@ Fixpoint teval(n: nat)(env: venv)(t: tm){struct n}: option (option vl) :=
     | 0 => None
     | S n =>
       match t with
-        | tvar x     => Some (index x env)
-        | tabs x T y => Some (Some (vabs env x T y))
-        | ttabs x T y  => Some (Some (vtabs env x T y))
+        | tvar x     => Some (indexr x env)
+        | tabs T y => Some (Some (vabs env T y))
+        | ttabs T y  => Some (Some (vtabs env T y))
         | tapp ef ex   =>
           match teval n env ex with
             | None => None
@@ -365,9 +341,9 @@ Fixpoint teval(n: nat)(env: venv)(t: tm){struct n}: option (option vl) :=
                 | None => None
                 | Some None => Some None
                 | Some (Some (vty _ _)) => Some None
-                | Some (Some (vtabs _ _ _ _)) => Some None
-                | Some (Some (vabs env2 x _ ey)) =>
-                  teval n ((x,vx)::env2) (open_tm (TVarF x) ey)
+                | Some (Some (vtabs _ _ _)) => Some None
+                | Some (Some (vabs env2 _ ey)) =>
+                  teval n (vx::env2) (open_tm (TVarF (length env2)) ey)
               end
           end
         | ttapp ef ex   =>
@@ -375,9 +351,9 @@ Fixpoint teval(n: nat)(env: venv)(t: tm){struct n}: option (option vl) :=
             | None => None
             | Some None => Some None
             | Some (Some (vty _ _)) => Some None
-            | Some (Some (vabs _ _ _ _)) => Some None
-            | Some (Some (vtabs env2 x T ey)) =>
-              teval n ((x,vty env ex)::env2) (open_tm (TVarF x) ey)
+            | Some (Some (vabs _ _ _)) => Some None
+            | Some (Some (vtabs env2 T ey)) =>
+              teval n ((vty env ex)::env2) (open_tm (TVarF (length env2)) ey)
           end
       end
   end.
@@ -388,7 +364,7 @@ Hint Unfold tenv.
 
 Hint Unfold open.
 Hint Unfold closed.
-Hint Unfold index.
+Hint Unfold indexr.
 Hint Unfold length.
 
 Hint Constructors ty.
@@ -430,13 +406,13 @@ Ltac crush2 :=
 
 Definition polyId := TAll TTop (TFun (TVarB 0) (TVarB 0)).
 
-Example ex1: has_type [] (ttabs 0 TTop (tabs 1 (TVarB 0) (tvar 1))) polyId.
+Example ex1: has_type [] (ttabs TTop (tabs (TVarB 0) (tvar 1))) polyId.
 Proof.
   crush_has_tp.
 Qed.
 
 (* instantiate it to TTop *)
-Example ex2: has_type [(0,polyId)] (ttapp (tvar 0) TTop) (TFun TTop TTop).
+Example ex2: has_type [polyId] (ttapp (tvar 0) TTop) (TFun TTop TTop).
 Proof.
   crush2.
 Qed.
@@ -448,16 +424,15 @@ Qed.
 
 (* ## Extension, Regularity ## *)
 
-Lemma wf_fresh : forall vs ts,
+Lemma wf_length : forall vs ts,
                     wf_env vs ts ->
-                    (fresh vs = fresh ts).
+                    (length vs = length ts).
 Proof.
   intros. induction H. auto.
   compute. eauto.
 Qed.
 
-Hint Immediate wf_fresh.
-
+Hint Immediate wf_length.
 
 Lemma wfh_length : forall vvs vs ts,
                     wf_envh vvs vs ts ->
@@ -467,29 +442,7 @@ Proof.
   compute. eauto.
 Qed.
 
-Hint Immediate wf_fresh.
-
-Lemma index_max : forall X vs n (T: X),
-                       index n vs = Some T ->
-                       n < fresh vs.
-Proof.
-  intros X vs. induction vs.
-  - Case "nil". intros. inversion H.
-  - Case "cons".
-    intros. inversion H. destruct a.
-    case_eq (le_lt_dec (fresh vs) i); intros ? E1.
-    + SCase "ok".
-      rewrite E1 in H1.
-      case_eq (beq_nat n i); intros E2.
-      * SSCase "hit".
-        eapply beq_nat_true in E2. subst n. compute. eauto.
-      * SSCase "miss".
-        rewrite E2 in H1.
-        assert (n < fresh vs). eapply IHvs. apply H1.
-        compute. omega.
-    + SCase "bad".
-      rewrite E1 in H1. inversion H1.
-Qed.
+Hint Immediate wfh_length.
 
 Lemma indexr_max : forall X vs n (T: X),
                        indexr n vs = Some T ->
@@ -498,7 +451,7 @@ Proof.
   intros X vs. induction vs.
   - Case "nil". intros. inversion H.
   - Case "cons".
-    intros. inversion H. destruct a.
+    intros. inversion H.
     case_eq (beq_nat n (length vs)); intros E2.
     + SSCase "hit".
       eapply beq_nat_true in E2. subst n. compute. eauto.
@@ -523,24 +476,9 @@ Proof. intros.
   intros. eauto.
 Qed.
 
-Lemma index_extend : forall X vs n n' x (T: X),
-                       index n vs = Some T ->
-                       fresh vs <= n' ->
-                       index n ((n',x)::vs) = Some T.
-
-Proof.
-  intros.
-  assert (n < fresh vs). eapply index_max. eauto.
-  assert (n <> n'). omega.
-  assert (beq_nat n n' = false) as E. eapply beq_nat_false_iff; eauto.
-  assert (fresh vs <= n') as E2. omega.
-  elim (le_xx (fresh vs) n' E2). intros ? EX.
-  unfold index. unfold index in H. rewrite H. rewrite E. rewrite EX. reflexivity.
-Qed.
-
-Lemma indexr_extend : forall X vs n n' x (T: X),
+Lemma indexr_extend : forall X vs n x (T: X),
                        indexr n vs = Some T ->
-                       indexr n ((n',x)::vs) = Some T.
+                       indexr n (x::vs) = Some T.
 
 Proof.
   intros.
@@ -548,7 +486,6 @@ Proof.
   assert (beq_nat n (length vs) = false) as E. eapply beq_nat_false_iff. omega.
   unfold indexr. unfold indexr in H. rewrite H. rewrite E. reflexivity.
 Qed.
-
 
 (* splicing -- for stp_extend. *)
 
@@ -563,17 +500,12 @@ Fixpoint splice n (T : ty) {struct T} : ty :=
     | TMem T0      => TMem (splice n T0)
   end.
 
-Definition splicett n (V: (id*ty)) :=
+Definition spliceat n (V: (venv*ty)) :=
   match V with
-    | (x,T) => (x,(splice n T))
+    | (G,T) => (G,splice n T)
   end.
 
-Definition spliceat n (V: (id*(venv*ty))) :=
-  match V with
-    | (x,(G,T)) => (x,(G,splice n T))
-  end.
-
-Lemma splice_open_permute: forall {X} (G0:list (id*X)) T2 n j,
+Lemma splice_open_permute: forall {X} (G0:list X) T2 n j,
 (open_rec j (TVarH (n + S (length G0))) (splice (length G0) T2)) =
 (splice (length G0) (open_rec j (TVarH (n + length G0)) T2)).
 Proof.
@@ -588,14 +520,14 @@ Proof.
   omega.
 Qed.
 
-Lemma indexr_splice_hi: forall G0 G2 x0 x v1 T,
+Lemma indexr_splice_hi: forall G0 G2 x0 v1 T,
     indexr x0 (G2 ++ G0) = Some T ->
     length G0 <= x0 ->
-    indexr (x0 + 1) (map (splicett (length G0)) G2 ++ (x, v1) :: G0) = Some (splice (length G0) T).
+    indexr (x0 + 1) (map (splice (length G0)) G2 ++ v1 :: G0) = Some (splice (length G0) T).
 Proof.
   intros G0 G2. induction G2; intros.
   - eapply indexr_max in H. simpl in H. omega.
-  - simpl in H. destruct a.
+  - simpl in H.
     case_eq (beq_nat x0 (length (G2 ++ G0))); intros E.
     + rewrite E in H. inversion H. subst. simpl.
       rewrite app_length in E.
@@ -607,10 +539,10 @@ Proof.
     + rewrite E in H.  eapply IHG2 in H. eapply indexr_extend. eapply H. eauto.
 Qed.
 
-Lemma indexr_spliceat_hi: forall G0 G2 x0 x v1 G T,
+Lemma indexr_spliceat_hi: forall G0 G2 x0 v1 G T,
     indexr x0 (G2 ++ G0) = Some (G, T) ->
     length G0 <= x0 ->
-    indexr (x0 + 1) (map (spliceat (length G0)) G2 ++ (x, v1) :: G0) =
+    indexr (x0 + 1) (map (spliceat (length G0)) G2 ++ v1 :: G0) =
     Some (G, splice (length G0) T).
 Proof.
   intros G0 G2. induction G2; intros.
@@ -624,7 +556,7 @@ Proof.
         eapply beq_nat_true_iff. eapply beq_nat_true_iff in E. omega.
       }
       rewrite H1. eauto.
-    + rewrite E in H.  eapply IHG2 in H. destruct p. eapply indexr_extend. eapply H. eauto.
+    + rewrite E in H.  eapply IHG2 in H. eapply indexr_extend. eapply H. eauto.
 Qed.
 
 Lemma plus_lt_contra: forall a b,
@@ -642,7 +574,7 @@ Lemma indexr_splice_lo0: forall {X} G0 G2 x0 (T:X),
 Proof.
   intros X G0 G2. induction G2; intros.
   - simpl in H. apply H.
-  - simpl in H. destruct a.
+  - simpl in H.
     case_eq (beq_nat x0 (length (G2 ++ G0))); intros E.
     + eapply beq_nat_true_iff in E. subst.
       rewrite app_length in H0. apply plus_lt_contra in H0. inversion H0.
@@ -655,7 +587,7 @@ Lemma indexr_extend_mult: forall {X} G0 G2 x0 (T:X),
 Proof.
   intros X G0 G2. induction G2; intros.
   - simpl. assumption.
-  - destruct a. simpl.
+  - simpl.
     case_eq (beq_nat x0 (length (G2 ++ G0))); intros E.
     + eapply beq_nat_true_iff in E.
       apply indexr_max in H. subst.
@@ -663,49 +595,24 @@ Proof.
     + apply IHG2. assumption.
 Qed.
 
-Lemma indexr_splice_lo: forall G0 G2 x0 x v1 T f,
+Lemma indexr_splice_lo: forall G0 G2 x0 v1 T f,
     indexr x0 (G2 ++ G0) = Some T ->
     x0 < length G0 ->
-    indexr x0 (map (splicett f) G2 ++ (x, v1) :: G0) = Some T.
+    indexr x0 (map (splice f) G2 ++ v1 :: G0) = Some T.
 Proof.
   intros.
   assert (indexr x0 G0 = Some T). eapply indexr_splice_lo0; eauto.
   eapply indexr_extend_mult. eapply indexr_extend. eauto.
 Qed.
 
-Lemma indexr_spliceat_lo: forall G0 G2 x0 x v1 G T f,
+Lemma indexr_spliceat_lo: forall G0 G2 x0 v1 G T f,
     indexr x0 (G2 ++ G0) = Some (G, T) ->
     x0 < length G0 ->
-    indexr x0 (map (spliceat f) G2 ++ (x, v1) :: G0) = Some (G, T).
+    indexr x0 (map (spliceat f) G2 ++ v1 :: G0) = Some (G, T).
 Proof.
   intros.
   assert (indexr x0 G0 = Some (G, T)). eapply indexr_splice_lo0; eauto.
   eapply indexr_extend_mult. eapply indexr_extend. eauto.
-Qed.
-
-
-Lemma fresh_splice_ctx: forall G n,
-  fresh G = fresh (map (splicett n) G).
-Proof.
-  intros. induction G.
-  - simpl. reflexivity.
-  - destruct a. simpl. reflexivity.
-Qed.
-
-Lemma index_splice_ctx: forall G x T n,
-  index x G = Some T ->
-  index x (map (splicett n) G) = Some (splice n T).
-Proof.
-  intros. induction G.
-  - simpl in H. inversion H.
-  - destruct a. simpl in H.
-    case_eq (le_lt_dec (fresh G) i); intros E LE; rewrite LE in H.
-    case_eq (beq_nat x i); intros Eq; rewrite Eq in H.
-    inversion H. simpl. erewrite <- (fresh_splice_ctx). rewrite LE.
-    rewrite Eq. reflexivity.
-    simpl. erewrite <- (fresh_splice_ctx). rewrite LE.
-    rewrite Eq. apply IHG. apply H.
-    inversion H.
 Qed.
 
 Lemma closed_splice: forall j l T n,
@@ -718,22 +625,21 @@ Proof.
   unfold closed. apply cl_selh. omega.
 Qed.
 
-Lemma map_splice_length_inc: forall G0 G2 x v1,
-   (length (map (splicett (length G0)) G2 ++ (x, v1) :: G0)) = (S (length (G2 ++ G0))).
+Lemma map_splice_length_inc: forall G0 G2 v1,
+   (length (map (splice (length G0)) G2 ++ v1 :: G0)) = (S (length (G2 ++ G0))).
 Proof.
   intros. rewrite app_length. rewrite map_length. induction G2.
   - simpl. reflexivity.
   - simpl. eauto.
 Qed.
 
-Lemma map_spliceat_length_inc: forall G0 G2 x v1,
-   (length (map (spliceat (length G0)) G2 ++ (x, v1) :: G0)) = (S (length (G2 ++ G0))).
+Lemma map_spliceat_length_inc: forall G0 G2 v1,
+   (length (map (spliceat (length G0)) G2 ++ v1 :: G0)) = (S (length (G2 ++ G0))).
 Proof.
   intros. rewrite app_length. rewrite map_length. induction G2.
   - simpl. reflexivity.
   - simpl. eauto.
 Qed.
-
 
 Lemma closed_inc: forall j l T,
   closed j l T ->
@@ -829,12 +735,12 @@ Proof.
   intros. apply (proj1 (stp2_closed G1 G2 T1 T2 GH H)).
 Qed.
 
-Lemma stp_splice : forall GX G0 G1 T1 T2 x v1,
+Lemma stp_splice : forall GX G0 G1 T1 T2 v1,
    stp GX (G1++G0) T1 T2 ->
-   stp GX ((map (splicett (length G0)) G1) ++ (x,v1)::G0)
+   stp GX ((map (splice (length G0)) G1) ++ v1::G0)
        (splice (length G0) T1) (splice (length G0) T2).
 Proof.
-  intros GX G0 G1 T1 T2 x v1 H. remember (G1++G0) as G.
+  intros GX G0 G1 T1 T2 v1 H. remember (G1++G0) as G.
   revert G0 G1 HeqG.
   induction H; intros; subst GH; simpl; eauto.
   - Case "sel1".
@@ -844,11 +750,11 @@ Proof.
     }
     rewrite <- A. apply IHstp. reflexivity.
   - Case "sela1".
-    case_eq (le_lt_dec (length G0) x0); intros E LE.
+    case_eq (le_lt_dec (length G0) x); intros E LE.
     + apply stp_sela1 with (T:=(splice (length G0) T)).
       assert (TMem (splice (length G0) T)=(splice (length G0) (TMem T))) as B by auto.
       rewrite B. apply indexr_splice_hi. eauto. eauto.
-      eapply closed_splice in H0. assert (S x0 = x0 +1) as A by omega.
+      eapply closed_splice in H0. assert (S x = x +1) as A by omega.
       rewrite <- A. eapply H0.
       eapply IHstp. eauto.
     + eapply stp_sela1. eapply indexr_splice_lo. eauto. eauto. eauto. eauto.
@@ -857,7 +763,7 @@ Proof.
       }
       rewrite <- A. eapply IHstp. eauto.
   - Case "selax".
-    case_eq (le_lt_dec (length G0) x0); intros E LE.
+    case_eq (le_lt_dec (length G0) x); intros E LE.
     + eapply stp_selax with (T:=splice (length G0) T).
       assert (TMem (splice (length G0) T)=(splice (length G0) (TMem T))) as B by auto.
       rewrite B. eapply indexr_splice_hi. eauto. eauto.
@@ -870,25 +776,25 @@ Proof.
 
     simpl. rewrite map_splice_length_inc. apply closed_splice. assumption.
 
-    specialize IHstp2 with (G3:=G0) (G4:=(0, TMem T1) :: G2).
+    specialize IHstp2 with (G3:=G0) (G4:=(TMem T1) :: G2).
     simpl in IHstp2. rewrite app_length. rewrite map_length. simpl.
-    repeat rewrite splice_open_permute with (j:=0). subst x0.
+    repeat rewrite splice_open_permute with (j:=0). subst x.
     rewrite app_length in IHstp2. simpl in IHstp2.
     eapply IHstp2. eauto.
 
-    specialize IHstp3 with (G3:=G0) (G4:=(0, TMem T3) :: G2).
+    specialize IHstp3 with (G3:=G0) (G4:=(TMem T3) :: G2).
     simpl in IHstp2. rewrite app_length. rewrite map_length. simpl.
-    repeat rewrite splice_open_permute with (j:=0). subst x0.
+    repeat rewrite splice_open_permute with (j:=0). subst x.
     rewrite app_length in IHstp3. simpl in IHstp3.
     eapply IHstp3. eauto.
 Qed.
 
-Lemma stp2_splice : forall G1 T1 G2 T2 GH1 GH0 x v1,
+Lemma stp2_splice : forall G1 T1 G2 T2 GH1 GH0 v1,
    stp2 G1 T1 G2 T2 (GH1++GH0) ->
    stp2 G1 (splice (length GH0) T1) G2 (splice (length GH0) T2)
-        ((map (spliceat (length GH0)) GH1) ++ (x,v1)::GH0).
+        ((map (spliceat (length GH0)) GH1) ++ v1::GH0).
 Proof.
-  intros G1 T1 G2 T2 GH1 GH0 x v1 H. remember (GH1++GH0) as GH.
+  intros G1 T1 G2 T2 GH1 GH0 v1 H. remember (GH1++GH0) as GH.
   revert GH0 GH1 HeqGH.
   induction H; intros; subst GH; simpl; eauto.
   - Case "sel1".
@@ -906,9 +812,9 @@ Proof.
     rewrite <- A. apply IHstp2.
     reflexivity.
   - Case "sela1".
-    case_eq (le_lt_dec (length GH0) x0); intros E LE.
+    case_eq (le_lt_dec (length GH0) x); intros E LE.
     + eapply stp2_sela1. eapply indexr_spliceat_hi. apply H. eauto.
-      eapply closed_splice in H0. assert (S x0 = x0 +1) by omega. rewrite <- H2.
+      eapply closed_splice in H0. assert (S x = x +1) by omega. rewrite <- H2.
       eapply H0.
       eapply IHstp2. eauto.
     + eapply stp2_sela1. eapply indexr_spliceat_lo. apply H. eauto. eauto.
@@ -917,7 +823,7 @@ Proof.
       }
       rewrite <- A. eapply IHstp2. eauto.
   - Case "selax".
-    case_eq (le_lt_dec (length GH0) x0); intros E LE.
+    case_eq (le_lt_dec (length GH0) x); intros E LE.
     + destruct v. eapply stp2_selax.
       eapply indexr_spliceat_hi. apply H. eauto.
     + destruct v. eapply stp2_selax.
@@ -930,24 +836,24 @@ Proof.
     simpl. rewrite map_spliceat_length_inc. apply closed_splice. assumption.
     simpl. rewrite map_spliceat_length_inc. apply closed_splice. assumption.
 
-    subst x0.
-    specialize IHstp2_2 with (GH2:=GH0) (GH3:=(0, (G1, T1)) :: GH1).
+    subst x.
+    specialize IHstp2_2 with (GH2:=GH0) (GH3:=(G1, T1) :: GH1).
     simpl in IHstp2_2.
     repeat rewrite splice_open_permute with (j:=0).
     rewrite app_length in IHstp2_2.
     eapply IHstp2_2. reflexivity.
 
-    subst x0.
-    specialize IHstp2_3 with (GH2:=GH0) (GH3:=(0, (G2, T3)) :: GH1).
+    subst x.
+    specialize IHstp2_3 with (GH2:=GH0) (GH3:=(G2, T3) :: GH1).
     simpl in IHstp2_3.
     repeat rewrite splice_open_permute with (j:=0).
     rewrite app_length in IHstp2_3.
     eapply IHstp2_3. reflexivity.
 Qed.
 
-Lemma stp_extend : forall G1 GH T1 T2 x v1,
+Lemma stp_extend : forall G1 GH T1 T2 v1,
                        stp G1 GH T1 T2 ->
-                       stp G1 ((x,v1)::GH) T1 T2.
+                       stp G1 (v1::GH) T1 T2.
 Proof.
   intros. induction H; eauto using indexr_extend.
   assert (splice (length GH) T2 = T2) as A2. {
@@ -969,15 +875,15 @@ Proof.
   assert (splice (length GH) T3 = T3) as A3. {
     eapply closed_splice_idem. eauto. omega.
   }
-  assert (map (splicett (length GH)) [(0,TMem T1)] ++(x,v1)::GH =
-          ((0,TMem T1)::(x,v1)::GH)) as HGX1. {
+  assert (map (splice (length GH)) [TMem T1] ++ v1::GH =
+          ((TMem T1)::v1::GH)) as HGX1. {
     simpl. rewrite A1. eauto.
   }
-  assert (map (splicett (length GH)) [(0,TMem T3)] ++(x,v1)::GH =
-          ((0,TMem T3)::(x,v1)::GH)) as HGX3. {
+  assert (map (splice (length GH)) [TMem T3] ++ v1::GH =
+          ((TMem T3)::v1::GH)) as HGX3. {
     simpl. rewrite A3. eauto.
   }
-  apply stp_all with (x:=length ((x,v1) :: GH)).
+  apply stp_all with (x:=length (v1 :: GH)).
   apply IHstp1.
   reflexivity.
   apply closed_inc. apply H1.
@@ -1000,27 +906,27 @@ Proof.
   simpl. unfold open in H4. rewrite <- H0. apply H4.
 Qed.
 
-Lemma indexr_at_index: forall {A} x0 GH0 GH1 x (v:A),
+Lemma indexr_at_index: forall {A} x0 GH0 GH1 (v:A),
   beq_nat x0 (length GH1) = true ->
-  indexr x0 (GH0 ++ (x, v) :: GH1) = Some v.
+  indexr x0 (GH0 ++ v :: GH1) = Some v.
 Proof.
   intros. apply beq_nat_true in H. subst.
   induction GH0.
   - simpl. rewrite <- beq_nat_refl. reflexivity.
-  - destruct a. simpl.
+  - simpl.
     rewrite app_length. simpl. rewrite <- plus_n_Sm. rewrite <- plus_Sn_m.
     rewrite false_beq_nat. assumption. omega.
 Qed.
 
-Lemma indexr_same: forall {A} x0 (v0:A) GH0 GH1 x (v:A) (v':A),
+Lemma indexr_same: forall {A} x0 (v0:A) GH0 GH1 (v:A) (v':A),
   beq_nat x0 (length GH1) = false ->
-  indexr x0 (GH0 ++ (x, v) :: GH1) = Some v0 ->
-  indexr x0 (GH0 ++ (x, v') :: GH1) = Some v0.
+  indexr x0 (GH0 ++ v :: GH1) = Some v0 ->
+  indexr x0 (GH0 ++ v' :: GH1) = Some v0.
 Proof.
-  intros ? ? ? ? ? ? ? ? E H.
+  intros ? ? ? ? ? ? ? E H.
   induction GH0.
   - simpl. rewrite E. simpl in H. rewrite E in H. apply H.
-  - destruct a. simpl.
+  - simpl.
     rewrite app_length. simpl.
     case_eq (beq_nat x0 (length GH0 + S (length GH1))); intros E'.
     simpl in H. rewrite app_length in H. simpl in H. rewrite E' in H.
@@ -1031,33 +937,22 @@ Qed.
 
 Inductive venv_ext : venv -> venv -> Prop :=
 | venv_ext_refl : forall G, venv_ext G G
-| venv_ext_cons : forall x T G1 G2, fresh G1 <= x -> venv_ext G1 G2 -> venv_ext ((x,T)::G1) G2.
+| venv_ext_cons : forall T G1 G2, venv_ext G1 G2 -> venv_ext (T::G1) G2.
 
 Inductive aenv_ext : aenv -> aenv -> Prop :=
 | aenv_ext_nil : aenv_ext nil nil
 | aenv_ext_cons :
-    forall x T G' G A A',
+    forall T G' G A A',
       aenv_ext A' A -> venv_ext G' G ->
-      aenv_ext ((x,(G',T))::A') ((x,(G,T))::A).
+      aenv_ext ((G',T)::A') ((G,T)::A).
 
 Lemma aenv_ext_refl: forall GH, aenv_ext GH GH.
 Proof.
   intros. induction GH.
   - apply aenv_ext_nil.
-  - destruct a. destruct p. apply aenv_ext_cons.
+  - destruct a. apply aenv_ext_cons.
     assumption.
     apply venv_ext_refl.
-Qed.
-
-Lemma index_extend_mult : forall G G' x T,
-                       index x G = Some T ->
-                       venv_ext G' G ->
-                       index x G' = Some T.
-Proof.
-  intros G G' x T H HV.
-  induction HV.
-  - assumption.
-  - apply index_extend. apply IHHV. apply H. assumption.
 Qed.
 
 Lemma aenv_ext__same_length:
@@ -1088,6 +983,16 @@ Proof.
     apply IHHext. assumption. assumption.
 Qed.
 
+Lemma indexr_extend_venv : forall G G' x T,
+                       indexr x G = Some T ->
+                       venv_ext G' G ->
+                       indexr x G' = Some T.
+Proof.
+  intros G G' x T H HV.
+  induction HV.
+  - assumption.
+  - apply indexr_extend. apply IHHV. apply H.
+Qed.
 
 Lemma stp2_closure_extend_rec :
   forall G1 G2 T1 T2 GH,
@@ -1103,17 +1008,17 @@ Proof.
   try solve [inversion IHstp2_1; inversion IHstp2_2; eauto];
   try solve [inversion IHstp2; eauto].
   - Case "sel1".
-    eapply stp2_sel1. eapply index_extend_mult. apply H.
+    eapply stp2_sel1. eapply indexr_extend_venv. apply H.
     assumption. assumption.
     apply IHstp2. assumption. apply venv_ext_refl. assumption.
   - Case "sel2".
-    eapply stp2_sel2. eapply index_extend_mult. apply H.
+    eapply stp2_sel2. eapply indexr_extend_venv. apply H.
     assumption. assumption.
     apply IHstp2. assumption. assumption. apply venv_ext_refl.
   - Case "selx".
     eapply stp2_selx.
-    eapply index_extend_mult. apply H. assumption.
-    eapply index_extend_mult. apply H0. assumption.
+    eapply indexr_extend_venv. apply H. assumption.
+    eapply indexr_extend_venv. apply H0. assumption.
   - Case "sela1".
     assert (exists GX', indexr x GH' = Some (GX', TX) /\ venv_ext GX' GX) as A. {
       apply indexr_at_ext with (GH:=GH); assumption.
@@ -1145,55 +1050,49 @@ Proof.
     apply IHstp2_3. apply aenv_ext_cons. assumption. assumption. assumption. assumption.
 Qed.
 
-Lemma stp2_closure_extend : forall G1 T1 G2 T2 GH GX T x v,
-                              stp2 G1 T1 G2 T2 ((0,(GX,T))::GH) ->
-                              fresh GX <= x ->
-                              stp2 G1 T1 G2 T2 ((0,((x,v)::GX,T))::GH).
+Lemma stp2_closure_extend : forall G1 T1 G2 T2 GH GX T v,
+                              stp2 G1 T1 G2 T2 ((GX,T)::GH) ->
+                              stp2 G1 T1 G2 T2 ((v::GX,T)::GH).
 Proof.
   intros. eapply stp2_closure_extend_rec. apply H.
   apply aenv_ext_cons. apply aenv_ext_refl. apply venv_ext_cons.
-  assumption. apply venv_ext_refl. apply venv_ext_refl. apply venv_ext_refl.
+  apply venv_ext_refl. apply venv_ext_refl. apply venv_ext_refl.
 Qed.
 
-Lemma stp2_extend : forall x v1 G1 G2 T1 T2 H,
+Lemma stp2_extend : forall v1 G1 G2 T1 T2 H,
                       stp2 G1 T1 G2 T2 H ->
-                      (fresh G1 <= x ->
-                       stp2 ((x,v1)::G1) T1 G2 T2 H) /\
-                      (fresh G2 <= x ->
-                       stp2 G1 T1 ((x,v1)::G2) T2 H) /\
-                      (fresh G1 <= x -> fresh G2 <= x ->
-                       stp2 ((x,v1)::G1) T1 ((x,v1)::G2) T2 H).
+                       stp2 (v1::G1) T1 G2 T2 H /\
+                       stp2 G1 T1 (v1::G2) T2 H /\
+                       stp2 (v1::G1) T1 (v1::G2) T2 H.
 Proof.
   intros. induction H0;
-    try solve [split; try split; intros; eauto using index_extend];
+    try solve [split; try split; intros; eauto using indexr_extend];
     try solve [split; try split; intros;
                inversion IHstp2_1 as [? [? ?]]; inversion IHstp2_2 as [? [? ?]]; eauto];
     try solve [split; try split; intros; inversion IHstp2 as [? [? ?]]; eauto];
-    try solve [split; try split; intros; inversion IHstp2 as [? [? ?]]; eauto using index_extend];
+    try solve [split; try split; intros; inversion IHstp2 as [? [? ?]]; eauto using indexr_extend];
     try solve [split; try split; intros; inversion IHstp2_1 as [? [? ?]];
                inversion IHstp2_2 as [? [? ?]]; inversion IHstp2_3 as [? [? ?]];
                eauto; eapply stp2_all; eauto using stp2_closure_extend].
 Qed.
 
-Lemma stp2_extend2 : forall x v1 G1 G2 T1 T2 H,
+Lemma stp2_extend2 : forall v1 G1 G2 T1 T2 H,
                        stp2 G1 T1 G2 T2 H ->
-                       fresh G2 <= x ->
-                       stp2 G1 T1 ((x,v1)::G2) T2 H.
+                       stp2 G1 T1 (v1::G2) T2 H.
 Proof.
-  intros. apply (proj2 (stp2_extend x v1 G1 G2 T1 T2 H H0)). assumption.
+  intros. apply (proj2 (stp2_extend v1 G1 G2 T1 T2 H H0)).
 Qed.
 
-Lemma stp2_extend1 : forall x v1 G1 G2 T1 T2 H,
+Lemma stp2_extend1 : forall v1 G1 G2 T1 T2 H,
                        stp2 G1 T1 G2 T2 H ->
-                       fresh G1 <= x ->
-                       stp2 ((x,v1)::G1) T1 G2 T2 H.
+                       stp2 (v1::G1) T1 G2 T2 H.
 Proof.
-  intros. apply (proj1 (stp2_extend x v1 G1 G2 T1 T2 H H0)). assumption.
+  intros. apply (proj1 (stp2_extend v1 G1 G2 T1 T2 H H0)).
 Qed.
 
-Lemma stp2_extendH : forall x v1 G1 G2 T1 T2 GH,
+Lemma stp2_extendH : forall v1 G1 G2 T1 T2 GH,
                        stp2 G1 T1 G2 T2 GH ->
-                       stp2 G1 T1 G2 T2 ((x,v1)::GH).
+                       stp2 G1 T1 G2 T2 (v1::GH).
 Proof.
   intros. induction H; eauto using indexr_extend.
   assert (splice (length GH) T2 = T2) as A2. {
@@ -1211,16 +1110,16 @@ Proof.
   assert (splice (length GH) T1 = T1) as A1. {
     eapply closed_splice_idem. eauto. omega.
   }
-  assert (map (spliceat (length GH)) [(0,(G1, T1))] ++(x,v1)::GH =
-          ((0, (G1, T1))::(x,v1)::GH)) as HGX1. {
+  assert (map (spliceat (length GH)) [(G1, T1)] ++ v1::GH =
+          ((G1, T1)::v1::GH)) as HGX1. {
     simpl. rewrite A1. eauto.
   }
   assert (closed 0 (length GH) T3). eapply stp2_closed1. eauto.
   assert (splice (length GH) T3 = T3) as A3. {
     eapply closed_splice_idem. eauto. omega.
   }
-  assert (map (spliceat (length GH)) [(0,(G2, T3))] ++(x,v1)::GH =
-          ((0, (G2, T3))::(x,v1)::GH)) as HGX3. {
+  assert (map (spliceat (length GH)) [(G2, T3)] ++ v1::GH =
+          ((G2, T3)::v1::GH)) as HGX3. {
     simpl. rewrite A3. eauto.
   }
   eapply stp2_all.
@@ -1236,7 +1135,7 @@ Proof.
   rewrite -> splice_open_permute.
   rewrite <- HGX1.
   apply stp2_splice.
-  subst x0. simpl. unfold open in H3. apply H3.
+  subst x. simpl. unfold open in H3. apply H3.
   simpl.
   rewrite <- A2. rewrite <- A4.
   unfold open.
@@ -1245,7 +1144,7 @@ Proof.
   rewrite -> splice_open_permute.
   rewrite <- HGX3.
   apply stp2_splice.
-  subst x0. simpl. unfold open in H4. apply H4.
+  subst x. simpl. unfold open in H4. apply H4.
 Qed.
 
 Lemma stp2_extendH_mult : forall G1 G2 T1 T2 H H2,
@@ -1254,7 +1153,7 @@ Lemma stp2_extendH_mult : forall G1 G2 T1 T2 H H2,
 Proof.
   intros. induction H2.
   - simpl. assumption.
-  - simpl. destruct a as [x v1].
+  - simpl.
     apply stp2_extendH. assumption.
 Qed.
 
@@ -1318,47 +1217,35 @@ Proof.
   intros. apply (proj1 (stp_reg G GH T1 T2 H)).
 Qed.
 
-Lemma valtp_extend : forall vs v x v1 T,
+Lemma valtp_extend : forall vs v v1 T,
                        val_type vs v T ->
-                       fresh vs <= x ->
-                       val_type ((x,v1)::vs) v T.
+                       val_type (v1::vs) v T.
 Proof.
   intros. induction H; eauto; econstructor; eauto; eapply stp2_extend2; eauto.
 Qed.
 
 
-Lemma index_safe_ex: forall H1 G1 TF i,
+Lemma indexr_safe_ex: forall H1 G1 TF i,
              wf_env H1 G1 ->
-             index i G1 = Some TF ->
-             exists v, index i H1 = Some v /\ val_type H1 v TF.
+             indexr i G1 = Some TF ->
+             exists v, indexr i H1 = Some v /\ val_type H1 v TF.
 Proof. intros. induction H.
    - Case "nil". inversion H0.
    - Case "cons". inversion H0.
-     case_eq (le_lt_dec (fresh ts) n); intros ? E1.
-     + SCase "ok".
-       rewrite E1 in H3.
-       assert ((fresh ts) <= n) as QF. eauto. rewrite <-(wf_fresh vs ts H1) in QF.
-       elim (le_xx (fresh vs) n QF). intros ? EX.
-
-       case_eq (beq_nat i n); intros E2.
-       * SSCase "hit".
-         assert (index i ((n, v) :: vs) = Some v). {
-           eauto. unfold index. rewrite EX. rewrite E2. eauto.
-         }
-         assert (t = TF).
-         unfold index in H0. rewrite E1 in H0. rewrite E2 in H0. inversion H0. eauto.
-         subst t. eauto.
-       * SSCase "miss".
-         rewrite E2 in H3.
-         assert (exists v0, index i vs = Some v0 /\ val_type vs v0 TF) as HI. {
-           eapply IHwf_env. eauto.
-         }
-         inversion HI as [v0 HI1]. inversion HI1.
-         eexists. econstructor. eapply index_extend; eauto. eapply valtp_extend; eauto.
-     + SSCase "bad".
-       rewrite E1 in H3. inversion H3.
+     case_eq (beq_nat i (length ts)); intros E2.
+     * SSCase "hit".
+       rewrite E2 in H3. inversion H3. subst. clear H3.
+       assert (length ts = length vs). symmetry. eapply wf_length. eauto.
+       simpl. rewrite H2 in E2. rewrite E2.
+       eexists. split. eauto. assumption.
+     * SSCase "miss".
+       rewrite E2 in H3.
+       assert (exists v0,
+                 indexr i vs = Some v0 /\ val_type vs v0 TF). eauto.
+       destruct H2. destruct H2.
+       eexists. split. eapply indexr_extend. eauto.
+       eapply valtp_extend. assumption.
 Qed.
-
 
 Lemma index_safeh_ex: forall H1 H2 G1 GH TF i,
              wf_env H1 G1 -> wf_envh H1 H2 GH ->
@@ -1408,8 +1295,10 @@ Proof.
   generalize dependent G.
   induction T2; intros G GH T1 S12; dependent induction S12;
   intros T3 S23; inversion S23; eauto 4 using stp_reg1, stp_reg2.
-  (* TAll - TAll *)
-  admit.
+  - (* TAll - TAll *)
+    subst.
+    eapply stp_all; eauto.
+    admit.
 Qed.
 
 Lemma stp2_trans: forall G1 G2 G3 T1 T2 T3 H,
@@ -1422,51 +1311,20 @@ Qed.
 
 (* ### Substitution for relating static and dynamic semantics ### *)
 
-Lemma index_miss {X}: forall x x1 (B:X) A G,
-  index x ((x1,B)::G) = A ->
-  fresh G <= x1 ->
-  x <> x1 ->
-  index x G = A.
-Proof.
-  intros.
-  unfold index in H.
-  elim (le_xx (fresh G) x1 H0). intros.
-  rewrite H2 in H.
-  assert (beq_nat x x1 = false). eapply beq_nat_false_iff. eauto.
-  rewrite H3 in H. eapply H.
-Qed.
 
-Lemma index_hit {X}: forall x x1 (B:X) A G,
-  index x ((x1,B)::G) = Some A ->
-  fresh G <= x1 ->
-  x = x1 ->
-  B = A.
-Proof.
-  intros.
-  unfold index in H.
-  elim (le_xx (fresh G) x1 H0). intros.
-  rewrite H2 in H.
-  assert (beq_nat x x1 = true). eapply beq_nat_true_iff. eauto.
-  rewrite H3 in H. inversion H. eauto.
-Qed.
-
-Lemma index_hit2 {X}: forall x x1 (B:X) A G,
-  fresh G <= x1 ->
-  x = x1 ->
+Lemma indexr_hit2 {X}: forall x (B:X) A G,
+  length G = x ->
   B = A ->
-  index x ((x1,B)::G) = Some A.
+  indexr x (B::G) = Some A.
 Proof.
   intros.
-  unfold index.
-  elim (le_xx (fresh G) x1 H). intros.
-  rewrite H2.
-  assert (beq_nat x x1 = true). eapply beq_nat_true_iff. eauto.
-  rewrite H3. rewrite H1. eauto.
+  unfold indexr.
+  assert (beq_nat x (length G) = true). eapply beq_nat_true_iff. eauto.
+  rewrite H1. subst. reflexivity.
 Qed.
 
-
-Lemma indexr_miss {X}: forall x x1 (B:X) A G,
-  indexr x ((x1,B)::G) = A ->
+Lemma indexr_miss {X}: forall x (B:X) A G,
+  indexr x (B::G) = A ->
   x <> (length G)  ->
   indexr x G = A.
 Proof.
@@ -1476,8 +1334,8 @@ Proof.
   rewrite H1 in H. eauto.
 Qed.
 
-Lemma indexr_hit {X}: forall x x1 (B:X) A G,
-  indexr x ((x1,B)::G) = Some A ->
+Lemma indexr_hit {X}: forall x (B:X) A G,
+  indexr x (B::G) = Some A ->
   x = length G ->
   B = A.
 Proof.
@@ -1487,9 +1345,8 @@ Proof.
   rewrite H1 in H. inversion H. eauto.
 Qed.
 
-
 Lemma indexr_hit0: forall GH (GX0:venv) (TX0:ty),
-      indexr 0 (GH ++ [(0,(GX0, TX0))]) =
+      indexr 0 (GH ++ [(GX0, TX0)]) =
       Some (GX0, TX0).
 Proof.
   intros GH. induction GH.
@@ -1654,28 +1511,22 @@ Proof.
   case_eq (beq_nat j i); intros E. eauto. eauto.
 Qed.
 
-(* substitution for one-env stp. not necessary, but good sanity check *)
-Definition substt (UX: ty) (V: (id*ty)) :=
-  match V with
-    | (x,T) => (x-1,(subst UX T))
-  end.
-
 Lemma indexr_subst: forall GH0 x TX T,
-   indexr x (GH0 ++ [(0, TMem TX)]) = Some T ->
+   indexr x (GH0 ++ [(TMem TX)]) = Some T ->
    x = 0 /\ TMem TX = T \/
-   x > 0 /\ indexr (x-1) (map (substt TX) GH0) = Some (subst TX T).
+   x > 0 /\ indexr (x-1) (map (subst TX) GH0) = Some (subst TX T).
 Proof.
   intros GH0. induction GH0; intros.
   - simpl in H. case_eq (beq_nat x 0); intros E.
     + rewrite E in H. inversion H.
       left. split. eapply beq_nat_true_iff. eauto. eauto.
     + rewrite E in H. inversion H.
-  -  destruct a. unfold id in H. remember ((length (GH0 ++ [(0, TMem TX)]))) as L.
+  -  unfold id in H. remember ((length (GH0 ++ [(TMem TX)]))) as L.
      case_eq (beq_nat x L); intros E.
      + assert (x = L). eapply beq_nat_true_iff. eauto.
        eapply indexr_hit in H.
        right. split. rewrite app_length in HeqL. simpl in HeqL. omega.
-       assert ((x - 1) = (length (map (substt TX) GH0))).
+       assert ((x - 1) = (length (map (subst TX) GH0))).
        rewrite map_length. rewrite app_length in HeqL. simpl in HeqL. unfold id. omega.
        simpl.
        eapply beq_nat_true_iff in H1. unfold id in H1. unfold id. rewrite H1.
@@ -1685,7 +1536,7 @@ Proof.
        inversion H. left. eapply H1.
        right. inversion H1. split. eauto.
        simpl.
-       assert ((x - 1) <> (length (map (substt TX) GH0))).
+       assert ((x - 1) <> (length (map (subst TX) GH0))).
        rewrite app_length in HeqL. simpl in HeqL. rewrite map_length.
        unfold not. intros. subst L. unfold id in H0. unfold id in H2.
        unfold not in H0. eapply H0. unfold id in H4. rewrite <-H4. omega.
@@ -1697,10 +1548,10 @@ Qed.
 Lemma stp_substitute: forall T1 T2 GX GH,
    stp GX GH T1 T2 ->
    forall GH0 TX,
-     GH = (GH0 ++ [(0,TMem TX)]) ->
+     GH = (GH0 ++ [(TMem TX)]) ->
      closed 0 0 TX ->
-     stp GX (map (substt TX) GH0) TX TX ->
-     stp GX (map (substt TX) GH0)
+     stp GX (map (subst TX) GH0) TX TX ->
+     stp GX (map (subst TX) GH0)
          (subst TX T1)
          (subst TX T2).
 Proof.
@@ -1748,7 +1599,7 @@ Proof.
     + rewrite map_length. eapply closed_subst. subst GH.
       rewrite app_length in H2. simpl in H2. eauto.
       eapply closed_upgrade_free; eauto. omega.
-    + specialize IHstp2 with (GH0:=(0, TMem T1)::GH0) (TX:=TX).
+    + specialize IHstp2 with (GH0:=(TMem T1)::GH0) (TX:=TX).
       subst GH. simpl in IHstp2.
       unfold open. unfold open in IHstp2.
       subst x.
@@ -1756,7 +1607,7 @@ Proof.
       rewrite app_length in IHstp2. simpl in IHstp2.
       eapply IHstp2; eauto. eapply stp_extend; eauto.
       eauto.
-    + specialize IHstp3 with (GH0:=(0, TMem T3)::GH0) (TX:=TX).
+    + specialize IHstp3 with (GH0:=(TMem T3)::GH0) (TX:=TX).
       subst GH. simpl in IHstp3.
       unfold open. unfold open in IHstp3.
       subst x.
@@ -1770,7 +1621,7 @@ Qed.
 (*
 when and how we can replace with multiple environments:
 
-stp2 G1 T1 G2 T2 (GH0 ++ [(0,vtya GX TX)])
+stp2 G1 T1 G2 T2 (GH0 ++ [(vty GX TX)])
 
 1) T1 closed
 
@@ -1794,17 +1645,16 @@ stp2 G1 T1 G2 T2 (GH0 ++ [(0,vtya GX TX)])
 (* ---- two-env substitution. first define what 'compatible' types mean. ---- *)
 
 Definition compat (GX:venv) (TX: ty) (G1:venv) (T1:ty) (T1':ty) :=
-  (exists x1, index x1 G1 = Some (vty GX TX) /\ T1' = (subst (TVarF x1) T1)) \/
+  (exists x1, indexr x1 G1 = Some (vty GX TX) /\ T1' = (subst (TVarF x1) T1)) \/
   (G1 = GX /\ T1' = (subst TX T1)) \/
   (closed 0 0 T1 /\ T1' = T1) \/ (* this one is for convenience: redundant with next *)
   (nosubst T1 /\ T1' = subst TTop T1).
 
 
-Definition compat2 (GX:venv) (TX: ty) (p1:id*(venv*ty)) (p2:id*(venv*ty)) :=
+Definition compat2 (GX:venv) (TX: ty) (p1:(venv*ty)) (p2:(venv*ty)) :=
   match p1, p2 with
-      (n1,(G1,T1)), (n2,(G2,T2)) => n1=n2(*+1 disregarded*) /\ G1 = G2 /\ compat GX TX G1 T1 T2
+      (G1,T1), (G2,T2) => G1 = G2 /\ compat GX TX G1 T1 T2
   end.
-
 
 Lemma closed_compat: forall GX TX GXX TXX TXX' j k,
   compat GX TX GXX TXX TXX' ->
@@ -1825,7 +1675,7 @@ Qed.
 
 Lemma indexr_compat_miss0: forall GH GH' GX TX (GXX:venv) (TXX:ty) n,
       Forall2 (compat2 GX TX) GH GH' ->
-      indexr (n+1) (GH ++ [(0,(GX, TX))]) = Some (GXX,TXX) ->
+      indexr (n+1) (GH ++ [(GX, TX)]) = Some (GXX,TXX) ->
       exists TXX', indexr n GH' = Some (GXX,TXX') /\ compat GX TX GXX TXX TXX'.
 Proof.
   intros. revert n H0. induction H.
@@ -1833,13 +1683,12 @@ Proof.
     eapply beq_nat_false_iff in H. rewrite H in H0. inversion H0.
   - intros. simpl. destruct y.
     case_eq (beq_nat n (length l')); intros E.
-    + simpl in H1. destruct x. rewrite app_length in H1. simpl in H1.
+    + simpl in H1. rewrite app_length in H1. simpl in H1.
       assert (n = length l'). eapply beq_nat_true_iff. eauto.
       assert (beq_nat (n+1) (length l + 1) = true). eapply beq_nat_true_iff.
       rewrite (Forall2_length _ _ _ _ _ H0). omega.
-      rewrite H3 in H1. destruct p. destruct p0. inversion H1. subst. simpl in H.
-      destruct H. destruct H2. subst. inversion H1. subst.
-      eexists. eauto.
+      rewrite H3 in H1. destruct x. inversion H1. subst. simpl in H.
+      destruct H. subst. eexists. eauto.
     + simpl in H1. destruct x.
       assert (n <> length l'). eapply beq_nat_false_iff. eauto.
       assert (beq_nat (n+1) (length l + 1) = false). eapply beq_nat_false_iff.
@@ -1903,7 +1752,7 @@ Lemma compat_sel: forall GX TX G1 T1' (GXX:venv) (TXX:ty) x,
     compat GX TX G1 (TVarF x) T1' ->
     closed 0 0 TX ->
     closed 0 0 TXX ->
-    index x G1 = Some (vty GXX TXX) ->
+    indexr x G1 = Some (vty GXX TXX) ->
     exists TXX', T1' = (TVarF x) /\ compat GX TX GXX TXX TXX'
 .
 Proof.
@@ -1919,7 +1768,7 @@ Qed.
 Lemma compat_selh: forall GX TX G1 T1' GH0 GH0' (GXX:venv) (TXX:ty) x,
     compat GX TX G1 (TVarH x) T1' ->
     closed 0 0 TX ->
-    indexr x (GH0 ++ [(0, (GX, TX))]) = Some (GXX, TXX) ->
+    indexr x (GH0 ++ [(GX, TX)]) = Some (GXX, TXX) ->
     Forall2 (compat2 GX TX) GH0 GH0' ->
     (x = 0 /\ GXX = GX /\ TXX = TX) \/
     exists TXX',
@@ -1982,7 +1831,7 @@ Qed.
 Lemma stp2_substitute: forall G1 G2 T1 T2 GH,
    stp2 G1 T1 G2 T2 GH ->
    forall GH0 GH0' GX TX T1' T2',
-     GH = (GH0 ++ [(0,(GX, TX))]) ->
+     GH = (GH0 ++ [(GX, TX)]) ->
      stp2 GX TX GX TX GH0' ->
      closed 0 0 TX ->
      compat GX TX G1 T1 T1' ->
@@ -2195,14 +2044,14 @@ Proof.
     + eauto.
     + eauto.
     + eauto.
-    + subst. specialize IHstp2_2 with (GH1 := (0, (G1, T1))::GH0).
+    + subst. specialize IHstp2_2 with (GH1 := (G1, T1)::GH0).
       eapply IHstp2_2.
       reflexivity.
       eapply stp2_extendH. eauto. eauto.
       rewrite app_length. simpl. rewrite EL. eauto.
       rewrite app_length. simpl. rewrite EL. eauto.
       eapply Forall2_cons. simpl. eauto. eauto.
-    + subst. specialize IHstp2_3 with (GH1 := (0, (G2, T3))::GH0).
+    + subst. specialize IHstp2_3 with (GH1 := (G2, T3)::GH0).
       eapply IHstp2_3.
       reflexivity.
       eapply stp2_extendH. eauto. eauto.
@@ -2227,8 +2076,8 @@ Proof.
   - Case "fun". eauto.
   - Case "mem". eauto.
   - Case "sel1".
-    assert (exists v : vl, index x GX = Some v /\ val_type GX v (TMem T)) as A.
-    eapply index_safe_ex. eauto. eauto.
+    assert (exists v : vl, indexr x GX = Some v /\ val_type GX v (TMem T)) as A.
+    eapply indexr_safe_ex. eauto. eauto.
     destruct A as [? [? VT]].
     inversion VT; try solve by inversion; subst.
     eapply stp2_sel1; eauto. inversion H2. subst.
@@ -2238,8 +2087,8 @@ Proof.
     eapply stp2_extendH_mult with (H2:=GY) in H8. rewrite app_nil_r in H8.
     eapply stp2_trans. eapply H8. eapply IHST; eauto.
   - Case "selx". eauto.
-    assert (exists v : vl, index x GX = Some v /\ val_type GX v (TMem T)) as A.
-    eapply index_safe_ex. eauto. eauto. eauto.
+    assert (exists v : vl, indexr x GX = Some v /\ val_type GX v (TMem T)) as A.
+    eapply indexr_safe_ex. eauto. eauto. eauto.
     destruct A as [? [? VT]].
     inversion VT; try solve by inversion; subst.
     inversion H2. subst.
@@ -2290,10 +2139,10 @@ Qed.
 Lemma invert_abs: forall venv vf T1 T2,
   val_type venv vf (TFun T1 T2) ->
   exists env tenv x y T3 T4,
-    vf = (vabs env x T3 y) /\
-    fresh env <= x /\
+    vf = (vabs env T3 y) /\
+    length env = x /\
     wf_env env tenv /\
-    has_type ((x,T3)::tenv) (open_tm (TVarF x) y) T4 /\
+    has_type (T3::tenv) (open_tm (TVarF x) y) T4 /\
     stp2 venv T1 env T3 [] /\
     stp2 env T4 venv T2 [].
 Proof.
@@ -2303,39 +2152,37 @@ Qed.
 Lemma invert_tabs: forall venv vf T1 T2,
   val_type venv vf (TAll T1 T2) ->
   exists env tenv x y T3 T4,
-    vf = (vtabs env x T3 y) /\
-    fresh env <= x /\
+    vf = (vtabs env T3 y) /\
+    length env = x /\
     wf_env env tenv /\
-    has_type ((x,TMem T3)::tenv) (open_tm (TVarF x) y) (open (TVarF x) T4) /\
+    has_type ((TMem T3)::tenv) (open_tm (TVarF x) y) (open (TVarF x) T4) /\
     stp2 venv T1 env T3 [] /\
-    stp2 ((x,vty venv T1)::env) (open (TVarF x) T4) venv (open T1 T2) [].
+    stp2 ((vty venv T1)::env) (open (TVarF x) T4) venv (open T1 T2) [].
 Proof.
   intros. inversion H; try solve by inversion. inversion H3. subst. repeat eexists; repeat eauto.
-  (*
-  remember (fresh venv1) as x.
-  remember (x + fresh venv0) as xx.
-  *)
+  remember (length venv1) as x.
 
   (* inversion of TAll < TAll *)
   assert (stp2 venv0 T1 venv1 T0 []). eauto.
-  assert (stp2 venv1 (open (TVarH 0) T3) venv0 (open (TVarH 0) T2) [(0,(venv0, T1))]). {
+  assert (stp2 venv1 (open (TVarH 0) T3) venv0 (open (TVarH 0) T2) [(venv0, T1)]). {
     eapply H19.
   }
 
   (* need reflexivity *)
   assert (stp2 venv0 T1 venv0 T1 []). eapply stp2_reg1. eauto.
-  assert (closed 0 0 T1). eapply stp2_closed1 in H6. simpl in H6. eauto.
+  assert (closed 0 0 T1). eapply stp2_closed1 in H5. simpl in H5. eauto.
 
   (* now rename *)
 
-  assert (stp2 ((x,vty venv0 T1) :: venv1) (open_rec 0 (TVarF x) T3) venv0 (open T1 T2) []). {
+  assert (stp2 ((vty venv0 T1) :: venv1) (open_rec 0 (TVarF x) T3) venv0 (open T1 T2) []). {
     eapply stp2_substitute with (GH0:=nil).
-    eapply stp2_extend1. eapply H5. eauto.
+    eapply stp2_extend1. eapply H4. simpl. eauto.
     simpl. eauto.
     eauto.
     eauto.
-    left. eexists. split. eapply index_hit2. eauto. eauto. eauto. unfold open.
-      rewrite (subst_open_zero 0 1). eauto. eauto.
+    left. eexists. split. eapply indexr_hit2. eauto. eauto. eauto. unfold open.
+    rewrite (subst_open_zero 0 1). subst x.
+    assert ((length venv1) + 0=length venv1) as R by omega. rewrite R. eauto. eauto.
     right. left. split. eauto. unfold open. rewrite (subst_open_zero 0 1). eauto. eauto.
     eauto.
   }
@@ -2359,14 +2206,14 @@ Proof.
 
   - Case "Var".
     remember (tvar i) as e. induction H0; inversion Heqe; subst.
-    + destruct (index_safe_ex venv0 env T1 i) as [v [I V]]; eauto.
+    + destruct (indexr_safe_ex venv0 env T1 i) as [v [I V]]; eauto.
       rewrite I. eapply not_stuck. eapply V.
 
     + eapply restp_widen. eapply IHhas_type; eauto. eapply stp_to_stp2; eauto. econstructor.
 
   - Case "Abs".
-    remember (tabs i t e) as xe. induction H0; inversion Heqxe; subst.
-    + eapply not_stuck. eapply v_abs; eauto. rewrite (wf_fresh venv0 env H1).
+    remember (tabs t e) as xe. induction H0; inversion Heqxe; subst.
+    + eapply not_stuck. eapply v_abs; eauto.
       eauto. eapply stp_to_stp2. eauto. eauto. econstructor.
     + eapply restp_widen. eapply IHhas_type; eauto. eapply stp_to_stp2; eauto. econstructor.
 
@@ -2389,7 +2236,7 @@ Proof.
           [env1 [tenv [x0 [y0 [T3 [T4 [EF [FRX [WF [HTY [STX STY]]]]]]]]]]]. eauto.
       (* now we know it's a closure, and we have has_type evidence *)
 
-      assert (res_type ((x0,vx)::env1) res T4) as HRY.
+      assert (res_type (vx::env1) res T4) as HRY.
         SCase "HRY".
           subst. eapply IHn. eauto. eauto.
           (* wf_env x *) econstructor. eapply valtp_widen; eauto.
@@ -2397,13 +2244,13 @@ Proof.
 
       inversion HRY as [? vy].
 
-      eapply not_stuck. eapply valtp_widen; eauto. eapply stp2_extend1. eauto. eauto.
+      eapply not_stuck. eapply valtp_widen; eauto. eapply stp2_extend1. eauto.
 
     + eapply restp_widen. eapply IHhas_type; eauto. eapply stp_to_stp2; eauto. econstructor.
 
   - Case "TAbs".
-    remember (ttabs i t e) as xe. induction H0; inversion Heqxe; subst.
-    + eapply not_stuck. eapply v_tabs; eauto. rewrite (wf_fresh venv0 env H1).
+    remember (ttabs t e) as xe. induction H0; inversion Heqxe; subst.
+    + eapply not_stuck. eapply v_tabs; eauto.
       eauto. eapply stp_to_stp2. eauto. eauto. econstructor.
     + eapply restp_widen. eapply IHhas_type; eauto. eapply stp_to_stp2; eauto. econstructor.
 
@@ -2422,7 +2269,7 @@ Proof.
           [env1 [tenv [x0 [y0 [T3 [T4 [EF [FRX [WF [HTY [STX STY]]]]]]]]]]]. eauto.
       (* now we know it's a closure, and we have has_type evidence *)
 
-      assert (res_type ((x0,vty venv0 T11)::env1) res (open (TVarF x0) T4)) as HRY.
+      assert (res_type ((vty venv0 T11)::env1) res (open (TVarF x0) T4)) as HRY.
         SCase "HRY".
           subst. eapply IHn. eauto. eauto.
           (* wf_env x *) econstructor. eapply v_ty.
